Main.lean
@@ -1,4 +1,4 @@
 import Demo
 
 def main : IO Unit :=
-  runtimeDemo
+  FromFile.runtimeDemo
